WIP

NuPrim.thy
@@ -18,6 +18,7 @@ theory NuPrim \<comment> \<open>The Primary Theory of the \<nu>-System\<close>
       and address = "\<^bold>a\<^bold>d\<^bold>d\<^bold>r\<^bold>e\<^bold>s\<^bold>s"
       and conversion = "\<^bold>c\<^bold>o\<^bold>n\<^bold>v\<^bold>e\<^bold>r\<^bold>s\<^bold>i\<^bold>o\<^bold>n"
       and auto = "\<^bold>a\<^bold>u\<^bold>t\<^bold>o"
+      and obligation = "\<^bold>o\<^bold>b\<^bold>l\<^bold>i\<^bold>g\<^bold>a\<^bold>t\<^bold>i\<^bold>o\<^bold>n"
 begin
 
 text \<open>The fundamental theory for \<nu>-system\<close>
@@ -352,7 +353,7 @@ subsubsection \<open>Elementary instructions\<close>
 
 definition bind :: " 'a state \<Rightarrow> ('a \<Rightarrow> 'b state) \<Rightarrow> 'b state " \<comment>\<open>monadic bind\<close>
   where "bind s f = (case s of StatOn x \<Rightarrow> f x | STrap \<Rightarrow> STrap | SNeg \<Rightarrow> SNeg)"
-definition instr_comp :: "('a \<Rightarrow> 'b state) \<Rightarrow> ('b \<Rightarrow> 'c state) \<Rightarrow> 'a \<Rightarrow> 'c state"  (infixr "\<nuInstrComp>" 75) 
+definition instr_comp :: "('a \<Rightarrow> 'b state) \<Rightarrow> ('b \<Rightarrow> 'c state) \<Rightarrow> 'a \<Rightarrow> 'c state"  ("_ \<nuInstrComp>/ _" [75,76] 75) 
   where "instr_comp f g s = bind (f s) g" \<comment>\<open>It is NOT monadic `then` operator (\<then>)!\<close>
 definition nop :: " 'a \<Rightarrow> 'a state" where "nop = StatOn" \<comment>\<open>the instruction `no-operation`\<close>
 definition call :: "('a \<Rightarrow> 'b state) \<Rightarrow> ('a \<flower> 'r) \<Rightarrow> ('b \<flower> 'r) state"
@@ -523,12 +524,11 @@ theorem start_construction: "CodeBlock s a S begin_proc_ctx \<Longrightarrow> (\
   unfolding begin_proc_ctx_def CodeBlock_def CurrentConstruction_def by (rule SpecTop_I; (rule NoFact)?) auto
 
 theorem finish_construction: "(\<And>a s. CodeBlock s a S f \<Longrightarrow> (\<^bold>c\<^bold>u\<^bold>r\<^bold>r\<^bold>e\<^bold>n\<^bold>t s \<^bold>r\<^bold>e\<^bold>s\<^bold>u\<^bold>l\<^bold>t\<^bold>s \<^bold>i\<^bold>n (T \<flower> R) \<^bold>w\<^bold>i\<^bold>t\<^bold>h \<^bold>f\<^bold>a\<^bold>c\<^bold>t\<^bold>s: PROP L))
-  \<Longrightarrow> f' = (f \<nuInstrComp> end_proc_ctx) \<Longrightarrow> \<^bold>p\<^bold>r\<^bold>o\<^bold>c f' \<blangle> S \<longmapsto> T \<brangle>" for S :: "'a set" and  T :: "('b::lrep) set" and  R :: "('c::register_collection) set"
+  \<Longrightarrow> \<^bold>p\<^bold>r\<^bold>o\<^bold>c (f \<nuInstrComp> end_proc_ctx) \<blangle> S \<longmapsto> T \<brangle>" for S :: "'a set" and  T :: "('b::lrep) set" and  R :: "('c::register_collection) set"
   unfolding CodeBlock_def Procedure_def
 proof
   assume rule:"(\<And>a s. a \<in> S \<and> f a = s \<and> s \<noteq> SNeg \<Longrightarrow> (\<^bold>c\<^bold>u\<^bold>r\<^bold>r\<^bold>e\<^bold>n\<^bold>t s \<^bold>r\<^bold>e\<^bold>s\<^bold>u\<^bold>l\<^bold>t\<^bold>s \<^bold>i\<^bold>n (T \<flower> R) \<^bold>w\<^bold>i\<^bold>t\<^bold>h \<^bold>f\<^bold>a\<^bold>c\<^bold>t\<^bold>s: PROP L))"
-    and def: "f' = f \<nuInstrComp> end_proc_ctx"
-  fix a show "a \<in> S \<longrightarrow> f' a \<in> \<S> T " unfolding def proof
+  fix a show "a \<in> S \<longrightarrow> (f \<nuInstrComp> end_proc_ctx) a \<in> \<S> T " proof
     assume a: "a \<in> S"
     moreover note rule[of a "f a", unfolded CurrentConstruction_def, simplified, THEN SpecTop_focus] 
     ultimately show "(f \<nuInstrComp> end_proc_ctx) a \<in> \<S> T" unfolding instr_comp_def bind_def end_proc_ctx_def
@@ -561,8 +561,10 @@ lemma [simp]: "((((\<^bold>c\<^bold>u\<^bold>r\<^bold>r\<^bold>e\<^bold>n\<^bold
 
 definition Cast :: " 'a set \<Rightarrow> 'a set \<Rightarrow> bool \<Rightarrow> bool " ("(2\<^bold>c\<^bold>a\<^bold>s\<^bold>t _ \<longmapsto> _/ \<^bold>m\<^bold>e\<^bold>a\<^bold>n\<^bold>w\<^bold>h\<^bold>i\<^bold>l\<^bold>e _)" [2,2,14] 13)
   where "(\<^bold>c\<^bold>a\<^bold>s\<^bold>t A \<longmapsto> B \<^bold>m\<^bold>e\<^bold>a\<^bold>n\<^bold>w\<^bold>h\<^bold>i\<^bold>l\<^bold>e P) \<longleftrightarrow> (\<forall>x. x \<in> A \<longrightarrow> x \<in> B \<and> P)"
-abbreviation SimpleCast :: " 'a set \<Rightarrow> 'a set \<Rightarrow> bool " ("(2\<^bold>c\<^bold>a\<^bold>s\<^bold>t _ \<longmapsto> _)" [2,14] 13)
-  where "(\<^bold>c\<^bold>a\<^bold>s\<^bold>t A \<longmapsto> B) \<equiv> (\<^bold>c\<^bold>a\<^bold>s\<^bold>t A \<longmapsto> B \<^bold>m\<^bold>e\<^bold>a\<^bold>n\<^bold>w\<^bold>h\<^bold>i\<^bold>l\<^bold>e True)"
+syntax SimpleCast :: " 'a set \<Rightarrow> 'a set \<Rightarrow> bool " ("(2\<^bold>c\<^bold>a\<^bold>s\<^bold>t _ \<longmapsto> _)" [2,14] 13)
+translations "(\<^bold>c\<^bold>a\<^bold>s\<^bold>t A \<longmapsto> B)" == "(\<^bold>c\<^bold>a\<^bold>s\<^bold>t A \<longmapsto> B \<^bold>m\<^bold>e\<^bold>a\<^bold>n\<^bold>w\<^bold>h\<^bold>i\<^bold>l\<^bold>e CONST True)"
+(* abbreviation SimpleCast :: " 'a set \<Rightarrow> 'a set \<Rightarrow> bool " ("(2\<^bold>c\<^bold>a\<^bold>s\<^bold>t _ \<longmapsto> _)" [2,14] 13)
+  where "(\<^bold>c\<^bold>a\<^bold>s\<^bold>t A \<longmapsto> B) \<equiv> (\<^bold>c\<^bold>a\<^bold>s\<^bold>t A \<longmapsto> B \<^bold>m\<^bold>e\<^bold>a\<^bold>n\<^bold>w\<^bold>h\<^bold>i\<^bold>l\<^bold>e True)" *)
 lemma Inhabited_subset: "Inhabited A \<Longrightarrow> A \<subseteq> B \<Longrightarrow> Inhabited B" unfolding Inhabited_def by auto
 lemma CastE[elim]: "\<^bold>c\<^bold>a\<^bold>s\<^bold>t A \<longmapsto> B \<^bold>m\<^bold>e\<^bold>a\<^bold>n\<^bold>w\<^bold>h\<^bold>i\<^bold>l\<^bold>e P \<Longrightarrow> (\<not> Inhabited A \<Longrightarrow> C) \<Longrightarrow> (Inhabited A \<Longrightarrow> Inhabited B \<Longrightarrow> A \<subseteq> B \<Longrightarrow> P \<Longrightarrow> C) \<Longrightarrow> C"
    unfolding Cast_def Inhabited_def by (auto intro: Inhabited_subset)
@@ -572,15 +574,20 @@ lemma [\<nu>cast]: "\<^bold>c\<^bold>a\<^bold>s\<^bold>t A \<longmapsto> A" by b
 lemma [\<nu>cast]: "\<^bold>c\<^bold>a\<^bold>s\<^bold>t A \<longmapsto> B \<^bold>m\<^bold>e\<^bold>a\<^bold>n\<^bold>w\<^bold>h\<^bold>i\<^bold>l\<^bold>e P \<Longrightarrow> \<^bold>c\<^bold>a\<^bold>s\<^bold>t \<S_S> A \<longmapsto> \<S_S> B \<^bold>m\<^bold>e\<^bold>a\<^bold>n\<^bold>w\<^bold>h\<^bold>i\<^bold>l\<^bold>e P" by blast
 lemma [\<nu>cast]: "\<^bold>c\<^bold>a\<^bold>s\<^bold>t A \<longmapsto> A' \<^bold>m\<^bold>e\<^bold>a\<^bold>n\<^bold>w\<^bold>h\<^bold>i\<^bold>l\<^bold>e P1 \<Longrightarrow> \<^bold>c\<^bold>a\<^bold>s\<^bold>t B \<longmapsto> B' \<^bold>m\<^bold>e\<^bold>a\<^bold>n\<^bold>w\<^bold>h\<^bold>i\<^bold>l\<^bold>e P2 \<Longrightarrow> \<^bold>c\<^bold>a\<^bold>s\<^bold>t (A\<boxbar>B) \<longmapsto> (A'\<boxbar>B') \<^bold>m\<^bold>e\<^bold>a\<^bold>n\<^bold>w\<^bold>h\<^bold>i\<^bold>l\<^bold>e P1 \<and> P2" by blast
 lemma LooseState_Cast[\<nu>cast]: "\<^bold>c\<^bold>a\<^bold>s\<^bold>t A \<longmapsto> B \<Longrightarrow> \<^bold>c\<^bold>a\<^bold>s\<^bold>t \<S> A \<longmapsto> \<S> B" unfolding \<nu>def Cast_def by auto
+lemma [\<nu>cast]: "\<^bold>c\<^bold>a\<^bold>s\<^bold>t A \<longmapsto> A' \<^bold>m\<^bold>e\<^bold>a\<^bold>n\<^bold>w\<^bold>h\<^bold>i\<^bold>l\<^bold>e P \<Longrightarrow> \<^bold>c\<^bold>a\<^bold>s\<^bold>t B \<longmapsto> B' \<^bold>m\<^bold>e\<^bold>a\<^bold>n\<^bold>w\<^bold>h\<^bold>i\<^bold>l\<^bold>e Q \<Longrightarrow> \<^bold>c\<^bold>a\<^bold>s\<^bold>t (A\<boxbar>B) \<longmapsto> (A'\<boxbar>B') \<^bold>m\<^bold>e\<^bold>a\<^bold>n\<^bold>w\<^bold>h\<^bold>i\<^bold>l\<^bold>e P \<and>Q"
+  unfolding Cast_def by auto
+
+definition Obligation :: "bool \<Rightarrow> bool" ("\<^bold>o\<^bold>b\<^bold>l\<^bold>i\<^bold>g\<^bold>a\<^bold>t\<^bold>i\<^bold>o\<^bold>n _" [10] 9) where "(\<^bold>o\<^bold>b\<^bold>l\<^bold>i\<^bold>g\<^bold>a\<^bold>t\<^bold>i\<^bold>o\<^bold>n P) \<longleftrightarrow> P"
+  \<comment> \<open>A tag to hint automatic provers to try to prove this proof obligation\<close>
+lemma [intro]: "P \<Longrightarrow> \<^bold>o\<^bold>b\<^bold>l\<^bold>i\<^bold>g\<^bold>a\<^bold>t\<^bold>i\<^bold>o\<^bold>n P" using Obligation_def by fast
+lemma [dest]: "\<^bold>o\<^bold>b\<^bold>l\<^bold>i\<^bold>g\<^bold>a\<^bold>t\<^bold>i\<^bold>o\<^bold>n P \<Longrightarrow> P" using Obligation_def by fast
+lemma [\<nu>cast]: "\<^bold>o\<^bold>b\<^bold>l\<^bold>i\<^bold>g\<^bold>a\<^bold>t\<^bold>i\<^bold>o\<^bold>n x = x' \<Longrightarrow> \<^bold>o\<^bold>b\<^bold>l\<^bold>i\<^bold>g\<^bold>a\<^bold>t\<^bold>i\<^bold>o\<^bold>n N = N' \<Longrightarrow>  \<^bold>c\<^bold>a\<^bold>s\<^bold>t (x \<tycolon> N) \<longmapsto> (x' \<tycolon> N')" unfolding Cast_def by fast
+lemma [\<nu>cast]: "\<^bold>o\<^bold>b\<^bold>l\<^bold>i\<^bold>g\<^bold>a\<^bold>t\<^bold>i\<^bold>o\<^bold>n x = x" by fast
 
 definition AutoTag :: "bool \<Rightarrow> bool" ("\<^bold>a\<^bold>u\<^bold>t\<^bold>o _" [100] 99) where [\<nu>def]: "\<^bold>a\<^bold>u\<^bold>t\<^bold>o P \<longleftrightarrow> P"
 lemma [\<nu>cast]: "\<^bold>c\<^bold>a\<^bold>s\<^bold>t U \<longmapsto> U' \<Longrightarrow> \<^bold>a\<^bold>u\<^bold>t\<^bold>o \<^bold>p\<^bold>r\<^bold>o\<^bold>c nop \<blangle> U \<longmapsto> U' \<brangle>"
   unfolding AutoTag_def Cast_def Procedure_def nop_def by auto
-
-ML \<open>fun f i = if i = 0 then raise Fail "" else f (i-1)
-val x = Runtime.exn_trace (fn _ => f 10)
-\<close>
-
+  
 definition Conversion :: "('a \<Rightarrow> 'b state) \<Rightarrow> 'a set \<Rightarrow> 'b set \<Rightarrow> ('c \<Rightarrow> 'd state) \<Rightarrow> 'c set \<Rightarrow> 'd set \<Rightarrow> bool" ("\<^bold>c\<^bold>o\<^bold>n\<^bold>v\<^bold>e\<^bold>r\<^bold>s\<^bold>i\<^bold>o\<^bold>n _/ (2\<blangle> _/ \<longmapsto> _ \<brangle>)/ \<long_dobule_mapsto> _/ (2\<blangle> _/ \<longmapsto> _ \<brangle>)" [101,2,2,101,2,2] 100)
   where [\<nu>def]: "\<^bold>c\<^bold>o\<^bold>n\<^bold>v\<^bold>e\<^bold>r\<^bold>s\<^bold>i\<^bold>o\<^bold>n f \<blangle> U \<longmapsto> V \<brangle> \<long_dobule_mapsto> g \<blangle> U' \<longmapsto> V' \<brangle> \<longleftrightarrow>( \<^bold>p\<^bold>r\<^bold>o\<^bold>c f \<blangle> U \<longmapsto> V \<brangle> \<longrightarrow> \<^bold>p\<^bold>r\<^bold>o\<^bold>c g \<blangle> U' \<longmapsto> V' \<brangle> )"
 lemma conversion_goal: "\<^bold>c\<^bold>o\<^bold>n\<^bold>v\<^bold>e\<^bold>r\<^bold>s\<^bold>i\<^bold>o\<^bold>n f \<blangle> U \<longmapsto> V \<brangle> \<long_dobule_mapsto> f' \<blangle> U' \<longmapsto> V' \<brangle> \<Longrightarrow> \<^bold>p\<^bold>r\<^bold>o\<^bold>c f \<blangle> U \<longmapsto> V \<brangle> \<Longrightarrow> \<^bold>p\<^bold>r\<^bold>o\<^bold>c f' \<blangle> U' \<longmapsto> V' \<brangle>"
@@ -588,8 +595,8 @@ lemma conversion_goal: "\<^bold>c\<^bold>o\<^bold>n\<^bold>v\<^bold>e\<^bold>r\<
 lemma [\<nu>cast]: "\<^bold>c\<^bold>o\<^bold>n\<^bold>v\<^bold>e\<^bold>r\<^bold>s\<^bold>i\<^bold>o\<^bold>n f \<blangle> U \<longmapsto> V \<brangle> \<long_dobule_mapsto> f \<blangle> U \<longmapsto> V \<brangle>" unfolding Conversion_def by fast
 lemma [\<nu>cast]: "\<^bold>c\<^bold>o\<^bold>n\<^bold>v\<^bold>e\<^bold>r\<^bold>s\<^bold>i\<^bold>o\<^bold>n f \<blangle> U \<longmapsto> V \<brangle> \<long_dobule_mapsto> g \<blangle> U' \<longmapsto> V' \<brangle> \<Longrightarrow> \<^bold>c\<^bold>o\<^bold>n\<^bold>v\<^bold>e\<^bold>r\<^bold>s\<^bold>i\<^bold>o\<^bold>n f \<blangle> U \<longmapsto> V \<brangle> \<long_dobule_mapsto> call g \<blangle> U' \<flower> W \<longmapsto> V' \<flower> W\<brangle>"
   unfolding Conversion_def using call by fast
-lemma [\<nu>cast]: "\<^bold>c\<^bold>a\<^bold>s\<^bold>t U' \<longmapsto> U \<Longrightarrow> \<^bold>c\<^bold>a\<^bold>s\<^bold>t V \<longmapsto> V' \<Longrightarrow> \<^bold>c\<^bold>o\<^bold>n\<^bold>v\<^bold>e\<^bold>r\<^bold>s\<^bold>i\<^bold>o\<^bold>n f \<blangle> U \<longmapsto> V \<brangle> \<long_dobule_mapsto> f \<blangle> U' \<longmapsto> V'\<brangle>"
-  unfolding Conversion_def Procedure_def Cast_def  by (auto dest: LooseState_Cast[unfolded Cast_def, simplified])
+lemma [\<nu>cast]: "\<^bold>c\<^bold>a\<^bold>s\<^bold>t U' \<longmapsto> U \<^bold>m\<^bold>e\<^bold>a\<^bold>n\<^bold>w\<^bold>h\<^bold>i\<^bold>l\<^bold>e P \<Longrightarrow> \<^bold>c\<^bold>a\<^bold>s\<^bold>t V \<longmapsto> V' \<^bold>m\<^bold>e\<^bold>a\<^bold>n\<^bold>w\<^bold>h\<^bold>i\<^bold>l\<^bold>e Q \<Longrightarrow> \<^bold>c\<^bold>o\<^bold>n\<^bold>v\<^bold>e\<^bold>r\<^bold>s\<^bold>i\<^bold>o\<^bold>n f \<blangle> U \<longmapsto> V \<brangle> \<long_dobule_mapsto> f \<blangle> U' \<longmapsto> V'\<brangle>"
+  unfolding Conversion_def Procedure_def Cast_def  by (auto 4 3 dest: LooseState_Cast[unfolded Cast_def, simplified])
 lemma [\<nu>cast]: "\<^bold>a\<^bold>u\<^bold>t\<^bold>o \<^bold>p\<^bold>r\<^bold>o\<^bold>c g \<blangle> U' \<longmapsto> U \<brangle> \<Longrightarrow> \<^bold>c\<^bold>o\<^bold>n\<^bold>v\<^bold>e\<^bold>r\<^bold>s\<^bold>i\<^bold>o\<^bold>n f \<blangle> U \<longmapsto> V \<brangle> \<long_dobule_mapsto> (g \<nuInstrComp> f) \<blangle> U' \<longmapsto> V\<brangle>"
   unfolding AutoTag_def Conversion_def using instr_comp by fast
 
